Complete proof ictr

ictr.fst
@@ -1,393 +1,109 @@
 module Ictr
 
-module L = FStar.List.Tot
+open FStar.Seq
 open FStar.Ghost
-open FStar.Seq.Base
-open FStar.Seq.Properties
 
-type op =
-  | Inc
+// the concrete state type
+// e.g. for the increment only counter (icounter), concrete_st = nat
+type concrete_st = nat
 
-type ctr_st = nat //concrete state of the counter
-type st = ctr_st & (erased (seq (ctr_st & (nat (*id*) & op))))
+// operation type
+// (the only operation is increment, so unit is fine)
+type op_t = unit
 
-val init : st
-let init = (0, hide empty)
+// apply an operation to a state
+let do (s:concrete_st) (_:log_entry) : concrete_st = s + 1
 
-val get_id : (nat * op) -> nat
-let get_id (id, o) = id
+let rec lem_foldl (s:concrete_st) (l:log)
+  : Lemma (ensures (seq_foldl do s l) = s + length l) 
+          (decreases length l)
+  = match length l with
+    |0 -> ()
+    |_ -> lem_foldl (do s (head l)) (tail l)
 
-val get_op : (ctr_st * (nat * op)) -> (nat * op)
-let get_op (_, o) = o
+//conflict resolution
+let resolve_conflict (x y:log_entry) : log =
+  cons x (cons y empty)
 
-val get_val : st -> ctr_st
-let get_val (c, _) = c
+let resolve_conflict_len (x y:log_entry)
+  : Lemma (Seq.length (resolve_conflict x y) = 2)
+  = ()
 
-val get_seq : st -> GTot (seq (ctr_st * (nat * op)))
-let get_seq (st, seq) = (reveal seq)
+let resolve_conflict_mem (x y:log_entry)
+  : Lemma (resolve_conflict_len x y;
+           let s = resolve_conflict x y in
+           (Seq.length s == 1 ==> is_x_or_y s x y) /\
+           (Seq.length s == 2 ==> is_x_and_y s x y))
+  = ()
 
-val get_st : (ctr_st * (nat * op)) -> ctr_st
-let get_st (st, o) = st
+// concrete merge pre-condition
+let concrete_merge_pre lca a b : prop
+  = a >= lca /\ b >= lca
 
-val get_init : c:st -> GTot nat
-let get_init c = 
-  if (length (get_seq c) > 0) then get_st (head (get_seq c)) else get_val c
+// concrete merge operation
+let concrete_merge (lca:concrete_st) (cst1:concrete_st) (cst2:concrete_st{concrete_merge_pre lca cst1 cst2}) 
+  : concrete_st = cst1 + cst2 - lca
 
-val last_op : c:st{length (get_seq c) > 0} -> GTot (nat * op)
-let last_op c = get_op (last (get_seq c))
+let merge_prop (lca s1 s2:st)
+  : Lemma (requires v_of lca == init_of s1 /\
+                    init_of s1 == init_of s2) 
+          (ensures concrete_merge_pre (v_of lca) (v_of s1) (v_of s2)) =
+  lem_foldl (init_of s1) (ops_of s1);
+  lem_foldl (init_of s2) (ops_of s2)
 
-val inverse : c:st{length (get_seq c) > 0} -> GTot ctr_st
-let inverse c = get_st (last (get_seq c))
+let merge_inv_prop (lca s1 s2:st)
+  : Lemma (requires length (ops_of s1) > 0 /\ length (ops_of s2) > 0 /\
+                    v_of lca == init_of s1 /\
+                    init_of s1 == init_of s2)
+          (ensures concrete_merge_pre (v_of lca) (v_of (inverse_st s1)) (v_of (inverse_st s2))) =
+  lem_foldl (init_of s1) (ops_of (inverse_st s1));
+  lem_foldl (init_of s2) (ops_of (inverse_st s2))
 
-val st_i : c:st{length (get_seq c) > 0} -> i:nat{i < length (get_seq c)} -> GTot ctr_st
-let st_i c i = (get_st (index (get_seq c) i))
+let linearizable_s1_0 (lca s1 s2:st)
+  : Lemma (requires 
+             v_of lca == init_of s1 /\
+             init_of s1 == init_of s2 /\
+             concrete_merge_pre (v_of lca) (v_of s1) (v_of s2) /\
+             length (ops_of s1) = 0) 
+          (ensures 
+             concrete_merge (v_of lca) (v_of s1) (v_of s2) ==
+             seq_foldl do (v_of lca) (ops_of s2)) =
+  ()
 
-val op_i : c:st{length (get_seq c) > 0} -> i:nat{i < length (get_seq c)} -> GTot (nat * op)
-let op_i c i = (get_op (index (get_seq c) i))
+let linearizable_s2_0 (lca s1 s2:st)
+  : Lemma (requires 
+             v_of lca == init_of s1 /\
+             init_of s1 == init_of s2 /\
+             concrete_merge_pre (v_of lca) (v_of s1) (v_of s2) /\
+             length (ops_of s2) = 0) 
+          (ensures 
+             concrete_merge (v_of lca) (v_of s1) (v_of s2) ==
+             seq_foldl do (v_of lca) (ops_of s1)) =
+  ()
 
-let pre_cond_do s op = true 
+let linearizable_s1s2_gt0 (lca s1 s2:st) (l':log)
+  : Lemma (requires 
+             v_of lca == init_of s1 /\
+             init_of s1 == init_of s2 /\
+             length (ops_of s1) > 0 /\ length (ops_of s2) > 0 /\
+             concrete_merge_pre (v_of lca) (v_of s1) (v_of s2) /\
+             concrete_merge_pre (v_of lca) (v_of (inverse_st s1)) (v_of (inverse_st s2)) /\
+             interleaving_predicate l' lca (inverse_st s1) (inverse_st s2))
+          (ensures 
+             (let l = Seq.append l' (resolve_conflict (last (ops_of s1)) (last (ops_of s2))) in
+               v_of (linearized_merge (v_of lca) l) == 
+               v_of (linearized_merge (v_of (linearized_merge (v_of lca) l'))
+                    (resolve_conflict (last (ops_of s1)) (last (ops_of s2)))) /\
 
-val do : c:ctr_st -> (nat * op) -> c1:ctr_st{c1 > c}
-let do c (_, Inc) = c + 1
+               concrete_merge (v_of lca) (v_of s1) (v_of s2) ==
+               v_of (linearized_merge (concrete_merge (v_of lca) (v_of (inverse_st s1)) (v_of (inverse_st s2))) 
+                    (resolve_conflict (last (ops_of s1)) (last (ops_of s2)))))) =
+    lem_foldl (init_of s1) (ops_of s1);
+    lem_foldl (init_of s2) (ops_of s2);
+    lem_foldl (init_of s1) (ops_of (inverse_st s1));
+    lem_foldl (init_of s2) (ops_of (inverse_st s2));
+    let l = Seq.append l' (resolve_conflict (last (ops_of s1)) (last (ops_of s2))) in
+    lem_foldl (v_of lca) l;
+    lem_foldl (v_of (linearized_merge (v_of lca) l')) (resolve_conflict (last (ops_of s1)) (last (ops_of s2)));
+    lem_foldl (v_of lca) l'
 
-val mem_id_l : id:nat -> s:(list (ctr_st & (nat (*id*) & op))) 
-             -> Tot (b:bool{(exists e. L.mem e s /\ get_id (get_op e) = id)  <==> (b = true)})
-let rec mem_id_l id s =
-  match s with
-  |[] -> false
-  |x::xs -> id = get_id (get_op x) || mem_id_l id xs
-
-val mem_id_s : id:nat -> c:(seq (ctr_st & (nat & op))) 
-           -> Tot (b:bool{(exists e. mem e c /\ get_id (get_op e) = id) <==> (b = true)})
-             (decreases length c)
-let rec mem_id_s id c = 
-  match length c with
-  |0 -> false
-  |_ -> id = get_id (get_op (head c)) || mem_id_s id (tail c)
-
-val mem_id : id:nat -> c:st
-           -> GTot (b:bool{(exists e. mem e (get_seq c) /\ get_id (get_op e) = id) <==> b = true})
-let mem_id id c = mem_id_s id (get_seq c)
-
-(*)val unique_id : (s:st) -> GTot bool
-                (decreases (length (get_seq s)))
-let rec unique_id s =
-  match length (get_seq s) with
-  |0 -> true
-  |_ -> (not (mem_id_s (get_id (get_op (head (get_seq s)))) (hide (tail (get_seq s))))) &&
-       (*unique_id (inverse s, hide (slice (get_seq s) 0 (length (get_seq s) - 1)))) &&*)
-       (unique_id (get_val s, (hide (tail (get_seq s)))))*)
-
-val unique_id_s : c:(seq (ctr_st & (nat & op)))  -> GTot bool
-                  (decreases (length c))
-let rec unique_id_s s =
-  match length s with
-  |0 -> true
-  |_ -> not (mem_id_s (get_id (get_op (head s))) (tail s)) && unique_id_s (tail s)
-
-val unique_id : (s:st) -> GTot bool
-let unique_id s = unique_id_s (get_seq s)
-
-val unique_id_l : s:(list (ctr_st & (nat & op))) 
-                -> Tot bool
-let rec unique_id_l s =
-  match s with
-  |[] -> true
-  |x::xs -> not (mem_id_l (get_id (get_op x)) xs) && unique_id_l xs
-
-(*)let unique_id (s:st) =
-  unique_id_l (seq_to_list (get_seq s))*)
-
-val count_id : id:nat -> s:seq(ctr_st & (nat (*id*) & op)) -> Tot nat (decreases length s)
-let rec count_id id s =
-  match length s with
-  |0 -> 0 
-  |_ -> if get_id (get_op (head s)) = id then 1 + count_id id (tail s) else count_id id (tail s)
-
-let valid_st (c:st) = 
-  (forall (i:nat). i < length (get_seq c) - 1 ==> (do (st_i c i) (op_i c i) = (st_i c (i+1)))) /\
-  (*forall (id:nat). mem_id id c ==> count_id id (get_seq c) = 1) /\*)
-  (forall (i:nat). i < length (get_seq c) - 1 ==> not (mem_id_s (get_id (op_i c i)) (slice (get_seq c) 0 i))
-            (*)not (mem_id_s (get_id (op_i c i)) (slice (get_seq c) 0 i)*)) /\
-  (length (get_seq c) > 0 ==> get_val c = do (inverse c) (last_op c)) 
-
-val to_unique_ls : l:(list (ctr_st & (nat (*id*) & op))) 
-              -> Lemma (requires true)
-                      (ensures (forall e. L.mem e l <==> mem e (seq_of_list l)) /\
-                               (unique_id_l l <==> unique_id_s (seq_of_list l)) /\ 
-                               L.length l = length (seq_of_list l))
-                      (decreases L.length l)
-#set-options "--z3rlimit 1000"
-let rec to_unique_ls l = 
-  lemma_seq_of_list_induction l;
-  match l with
-  |[] -> ()
-  |x::xs -> to_unique_ls xs
-  
-(*)val rem_last : s:(seq (ctr_st & (nat & op))){length s > 0 /\ unique_id_s s}
-             -> Pure (seq (ctr_st & (nat & op)))
-               (requires length s > 0 /\ unique_id_s s)
-               (ensures (fun s1 -> (length s1 = length s - 1) /\
-                                (forall e. mem e s /\ e <> last s <==> mem e s1)
-                                (*forall id. mem_id_s id s <==> mem_id_s id s1 \/ id = get_id (get_op (last s))*)))
-               (decreases length s)
-
-#set-options "--z3rlimit 1000"
-let rem_last s = 
-  match length s with
-  |1 -> empty
-  |_ -> slice s 0 (length s - 1)*)
- 
-val to_unique_sl : s:(seq (ctr_st & (nat & op)))
-                -> Lemma (requires true)
-                        (ensures (forall e. mem e s <==> L.mem e (seq_to_list s))  /\
-                                 (unique_id_s s <==> unique_id_l (seq_to_list s)) /\ 
-                                 length s = L.length (seq_to_list s) /\
-                                 (length s > 0 ==> (forall e. mem e (slice s 0 (length s - 1)) ==> mem e s) /\
-                                         (length (slice s 0 (length s - 1)) = length s - 1) /\
-                                 (forall id. mem_id_s id (slice s 0 (length s - 1)) ==> mem_id_s id s)))
-                        (decreases length s)
-
-#set-options "--z3rlimit 1000"
-let rec to_unique_sl s = 
-  match length s with
-  |0 -> ()
-  |_ ->  to_unique_sl (tail s)
-
-val init_le_inv : c:st
-           -> Lemma (requires valid_st c /\ length (get_seq c) > 0)
-                   (ensures get_init c <= inverse c /\ get_val c = get_init c + length (get_seq c))
-                   (decreases (length (get_seq c)))
-
-#set-options "--z3rlimit 1000"
-let rec init_le_inv c = 
-  match (length (get_seq c)) with
-  |0 -> ()
-  |1 -> ()
-  |_ -> init_le_inv (inverse c, hide (slice (get_seq c) 0 (length (get_seq c) - 1)))
-
-val pre_cond_merge : l:ctr_st -> a:ctr_st -> b:ctr_st -> bool
-let pre_cond_merge l a b = a >= l && b >= l
-
-val merge : l:ctr_st -> a:ctr_st -> b:ctr_st
-           -> Pure ctr_st (requires pre_cond_merge l a b)
-                    (ensures (fun r -> r = a + b - l))
-let merge l a b =
-  a + b - l
-
-//equivalence relation between 2 states
-val eq_m : a:ctr_st -> b:ctr_st -> bool
-let eq_m a b = a = b
-
-(*)val spec : ctr_st -> (nat * op) -> (nat * op) -> nat
-let spec a o1 o2 =
-    do (do a o1) o2*)
-
-val mem_op_s : o:(nat * op) -> s:(seq (ctr_st & (nat & op))) 
-             -> Tot (b:bool{(exists e. mem e s /\ get_op e = o)  <==> (b = true)})
-             (decreases length s)
-let rec mem_op_s o s =
-  match length s with
-  |0 -> false
-  |_ -> get_op (head s) = o || mem_op_s o (tail s)
-
-let mem_op (o:(nat * op)) (s:st) =
-  mem_op_s o (get_seq s)
-
-(*)val lem_spec : l:st -> a:st -> b:st
-             -> o1:(nat * op) -> o2:(nat * op)
-             -> Lemma (requires get_id o1 <> get_id o2 /\
-                               (get_val a) = do (get_val l) o1 /\ (get_val b) = do (get_val l) o2)
-                     (ensures pre_cond_merge (get_val l) (get_val a) (get_val b) /\ 
-                              eq_m (spec (get_val l) o1 o2) (merge (get_val l) (get_val a) (get_val b)) /\
-                              (exists (s:st). valid_st s /\ get_init s = get_val l /\
-                              (forall o. mem_op o s <==> o = o1 \/ o = o2) /\
-                              eq_m (merge (get_val l) (get_val a) (get_val b)) (get_val s)))
-
-#set-options "--z3rlimit 1000"
-let lem_spec l a b o1 o2 = 
-  let s = (spec (get_val l) o1 o2, hide (cons (get_val l, o1) (create 1 (do (get_val l) o1, o2)))) in
-  assert (valid_st s /\ eq_m (merge (get_val l) (get_val a) (get_val b)) (get_val s));
-  ()*)
-
-val spec : a:ctr_st -> o1:(nat * op) -> o2:(nat * op){get_id o1 <> get_id o2} -> s:st{valid_st s}
-let spec a o1 o2 =
-  (do (do a o1) o2 , hide (cons (a, o1) (cons (do a o1, o2) empty))) 
-
-val lem_spec : l:st -> a:st -> b:st
-             -> o1:(nat * op) -> o2:(nat * op)
-             -> Lemma (requires pre_cond_do (get_val l) o1 /\ pre_cond_do (get_val l) o2 /\ get_id o1 <> get_id o2 /\ 
-                               valid_st l /\ valid_st a /\ valid_st b /\
-                               length (get_seq a) > 0 /\ length (get_seq b) > 0 /\
-                               get_val a = do (get_val l) o1 /\ get_val b = do (get_val l) o2 /\
-                               pre_cond_merge (get_val l) (get_val a) (get_val b) )
-                     (ensures (*)pre_cond_merge (get_val l) (get_val a) (get_val b) /\ *)
-                         eq_m (get_val (spec (get_val l) o1 o2)) (merge (get_val l) (get_val a) (get_val b)) /\
-
-                              (exists (s:st). valid_st s /\ get_init s = get_val l /\
-                                (forall o. mem_op o s <==> o = o1 \/ o = o2) /\
-                                      eq_m (merge (get_val l) (get_val a) (get_val b)) (get_val s)))
-
-#set-options "--z3rlimit 100000"
-let lem_spec l a b o1 o2 = 
-  (*)init_le_inv a; init_le_inv b;*)
-  let s = spec (get_val l) o1 o2 in 
-  introduce exists s. valid_st s /\ get_init s = get_val l /\ (forall o. mem_op o s <==> o = o1 \/ o = o2) /\
-                   eq_m (merge (get_val l) (get_val a) (get_val b)) (get_val s)
-  with s
-  and ()
-
-val len_ab_gt0 : l:st -> a:st -> b:st
-                -> Lemma (requires valid_st l /\ valid_st a /\ valid_st b /\
-                                  length (get_seq a) > 0 /\ length (get_seq b) > 0 /\
-                                  get_init a = get_init b /\ get_init a = get_val l /\ 
-                                  pre_cond_merge (get_val l) (get_val a) (get_val b) /\
-                                  (forall id. mem_id id l ==> not (mem_id id a)) /\
-                                  (forall id. mem_id id a ==> not (mem_id id b)) /\
-                                  (forall id. mem_id id l ==> not (mem_id id b)))
-                         (ensures pre_cond_merge (get_val l) (inverse a) (inverse b) /\
-                                  (let m = merge (get_val l) (inverse a) (inverse b) in
-                                       eq_m (merge (get_val l) (get_val a) (get_val b))
-                                            (*merge m (do m (last_op a)) (do m (last_op b))*)
-                                            (do (do m (last_op a)) (last_op b)) /\
-
-                                  (exists (s:st). valid_st s /\ get_init s = m /\
-                                     (forall o. mem_op o s <==> o = last_op a \/ o = last_op b) /\ 
-                                     eq_m (merge (get_val l) (get_val a) (get_val b)) (get_val s))))
-
-#set-options "--z3rlimit 10000"
-let len_ab_gt0 l a b =
-  init_le_inv a;
-  init_le_inv b;
-  let m = merge (get_val l) (inverse a) (inverse b) in
-  let s = ((do (do m (last_op a)) (last_op b)), hide (cons (m, last_op a) (cons (do m (last_op a), last_op b) empty))) in
-  assume (valid_st s);
-  assume (eq_m (merge (get_val l) (get_val a) (get_val b))
-               (do (do m (last_op a)) (last_op b)));
-  assume (get_init s = m); 
-  assume (get_id (last_op a) <> get_id (last_op b)); 
-  assume (forall o. mem_op o s ==> o = last_op a \/ o = last_op b);
-  assume (forall o. o = last_op a \/ o = last_op b ==> mem_op o s); 
-  assert (forall o. o = last_op a \/ o = last_op b <==> mem_op o s);
-  introduce exists s. valid_st s /\ get_init s = m /\ (forall o. mem_op o s <==> o = last_op a \/ o = last_op b) /\ 
-          eq_m (merge (get_val l) (get_val a) (get_val b)) (get_val s)
-  with s
-  and ()
-
-val len_b_gt0 : l:st -> a:st -> b:st
-                -> Lemma (requires valid_st l /\ valid_st a /\ valid_st b /\ 
-                                  length (get_seq a) = 0 /\ length (get_seq b) > 0 /\
-                                  get_init a = get_init b /\ get_init a = get_val l /\ 
-                                  pre_cond_merge (get_val l) (get_val a) (get_val b) /\
-                                  (forall id. mem_id id l ==> not (mem_id id a)) /\
-                                  (forall id. mem_id id a ==> not (mem_id id b)) /\
-                                  (forall id. mem_id id l ==> not (mem_id id b)))
-                         (ensures pre_cond_merge (get_val l) (get_val a) (inverse b) /\
-                                 (let m = merge (get_val l) (get_val a) (inverse b) in
-                                      eq_m (merge (get_val l) (get_val a) (get_val b)) 
-                                           (do m (last_op b)) /\
-
-                                 (exists (s:st). valid_st s /\ get_init s = m /\
-                                    (forall o. mem_op o s <==> o = last_op b) /\ 
-                                    eq_m (merge (get_val l) (get_val a) (get_val b)) (get_val s))))
-
-#set-options "--z3rlimit 1000"
-let len_b_gt0 l a b = 
-  init_le_inv b;
-  let m = merge (get_val l) (get_val a) (inverse b) in
-  let s = ((do m (last_op b)), hide (cons (m, last_op b) empty)) in
-  introduce exists s. valid_st s /\ get_init s = m /\ (forall o. mem_op o s <==> o = last_op b) /\ 
-          eq_m (merge (get_val l) (get_val a) (get_val b)) (get_val s)
-  with s
-  and ()
-
-val len_a_gt0 : l:st -> a:st -> b:st
-                -> Lemma (requires valid_st l /\ valid_st a /\ valid_st b /\ 
-                                  length (get_seq a) > 0 /\ length (get_seq b) = 0 /\
-                                  get_init a = get_init b /\ get_init a = get_val l /\ 
-                                  pre_cond_merge (get_val l) (get_val a) (get_val b) /\
-                                  (forall id. mem_id id l ==> not (mem_id id a)) /\
-                                  (forall id. mem_id id a ==> not (mem_id id b)) /\
-                                  (forall id. mem_id id l ==> not (mem_id id b)))
-                        (ensures pre_cond_merge (get_val l) (inverse a) (get_val b) /\
-                                 (let m = merge (get_val l) (inverse a) (get_val b) in
-                                      eq_m (merge (get_val l) (get_val a) (get_val b))
-                                           (do m (last_op a)) /\
-
-                                 (exists (s:st). valid_st s /\ get_init s = m /\
-                                    (forall o. mem_op o s <==> o = last_op a) /\ 
-                                    eq_m (merge (get_val l) (get_val a) (get_val b)) (get_val s))))
-
-#set-options "--z3rlimit 1000"
-let len_a_gt0 l a b =
-  init_le_inv a;
-  let m = merge (get_val l) (inverse a) (get_val b) in
-  let s = ((do m (last_op a)), hide (cons (m, last_op a) empty)) in
-  introduce exists s. valid_st s /\ get_init s = m /\ (forall o. mem_op o s <==> o = last_op a) /\ 
-          eq_m (merge (get_val l) (get_val a) (get_val b)) (get_val s)
-  with s
-  and ()
-
-val len_ab_0 : l:st -> a:st -> b:st
-                -> Lemma (requires valid_st l /\ valid_st a /\ valid_st b /\ 
-                                  length (get_seq a) = 0 /\ length (get_seq b) = 0 /\
-                                  get_init a = get_init b /\ get_init a = get_val l /\ 
-                                  pre_cond_merge (get_val l) (get_val a) (get_val b) /\
-                                  (forall id. mem_id id l ==> not (mem_id id a)) /\
-                                  (forall id. mem_id id a ==> not (mem_id id b)) /\
-                                  (forall id. mem_id id l ==> not (mem_id id b)))
-                        (ensures (eq_m (merge (get_val l) (get_val a) (get_val b)) (get_val l)) /\
-
-                                 (exists (s:st). valid_st s /\ get_init s = get_val l /\ length (get_seq s) = 0 /\
-                                    eq_m (merge (get_val l) (get_val a) (get_val b)) (get_val s)))
-
-#set-options "--z3rlimit 1000"
-let len_ab_0 l a b = ()
-
-val final : l:st -> a:st -> b:st
-          -> Lemma (requires valid_st l /\ valid_st a /\ valid_st b /\
-                            get_init a = get_init b /\ get_init a = get_val l /\
-                            pre_cond_merge (get_val l) (get_val a) (get_val b) /\
-                            (forall id. mem_id id l ==> not (mem_id id a)) /\
-                            (forall id. mem_id id a ==> not (mem_id id b)) /\
-                            (forall id. mem_id id l ==> not (mem_id id b)))
-                  (ensures (exists (s:st). valid_st s /\ get_init s = get_val l /\
-                                      (forall o. mem_op o s <==> mem_op o a \/ mem_op o b) /\ 
-                                      eq_m (merge (get_val l) (get_val a) (get_val b)) (get_val s)))
-                  (decreases %[length (get_seq a); length (get_seq b)])
-
-#set-options "--initial_fuel 0 --max_fuel 10 --initial_ifuel 0 --max_ifuel 10 --z3rlimit 10000"
-let rec final l a b =
-    match length (get_seq a), length (get_seq b) with
-    |0,0 -> len_ab_0 l a b
-    
-    |1,0 -> admit();introduce exists s. valid_st s /\ get_init s = get_val l /\ (forall o. mem_op o s <==> mem_op o a \/ mem_op o b) /\
-           eq_m (merge (get_val l) (get_val a) (get_val b)) (get_val s) 
-           with ((do (merge (get_val l) (inverse a) (get_val b)) (last_op a)), 
-                     hide (cons ((merge (get_val l) (inverse a) (get_val b)), last_op a) empty))
-           and ()
-
-    |0,1 -> admit();introduce exists s. valid_st s /\ get_init s = get_val l /\ (forall o. mem_op o s <==> mem_op o a \/ mem_op o b) /\ 
-           eq_m (merge (get_val l) (get_val a) (get_val b)) (get_val s)
-           with ((do (merge (get_val l) (get_val a) (inverse b)) (last_op b)), 
-                     hide (cons ((merge (get_val l) (get_val a) (inverse b)), last_op b) empty))
-           and ()
-
-    |1,1 -> admit();len_ab_gt0 l a b;
-           assert (exists (s:st). valid_st s /\ get_init s = (merge (get_val l) (inverse a) (inverse b)) /\
-                     (forall o. mem_op o s <==> o = last_op a \/ o = last_op b) /\ 
-                     eq_m (merge (get_val l) (get_val a) (get_val b)) (get_val s)); 
-           final l (inverse a, hide (slice (get_seq a) 0 (length (get_seq a) - 1)))
-                   (inverse b, hide (slice (get_seq b) 0 (length (get_seq b) - 1)))
-
-    |0,_ -> len_b_gt0 l a b; 
-           assume (exists (s:st). valid_st s /\ get_init s = (merge (get_val l) (get_val a) (inverse b)) /\
-                     (forall o. mem_op o s <==> o = last_op b) /\ 
-                     eq_m (merge (get_val l) (get_val a) (get_val b)) (get_val s)); 
-           final l a (inverse b, hide (slice (get_seq b) 0 (length (get_seq b) - 1)))
-    |_,0 -> admit(); len_a_gt0 l a b; final l (inverse a, hide (slice (get_seq a) 0 (length (get_seq a) - 1))) b
-    |_,_ -> admit(); len_ab_gt0 l a b; final l (inverse a, hide (slice (get_seq a) 0 (length (get_seq a) - 1)))
-                                     (inverse b, hide (slice (get_seq b) 0 (length (get_seq b) - 1)))
-
-    
- 
